parametric/Parametric1.lean
@@ -60,8 +60,8 @@ theorem lift_map (g : α → β) : ∀ l, lift (λ x y => g x = y) l (l.map g)
   | [] => trivial
   | _::l => ⟨rfl, lift_map g l⟩
 
-instance : ParaF λ α => List (α i) where
-  prop _ _ r := lift (r i)
+instance [ParaF ϕ] : ParaF λ α => List (ϕ α) where
+  prop α β r := lift (ParaF.prop α β r)
 
 example : ParaT.prop (@f : ∀ {α β}, (α → β → β) → β → List α → β) =
   ∀ {α α'} (r : α → α' → Prop) {β β'} (s : β → β' → Prop),
@@ -80,5 +80,13 @@ example : ParaT.prop (@List.foldr) := by
 
 example (f : Para (∀ {α β}, (α → β → β) → β → List α → β)) (g : α → α') (h : β → β') (c c') (hc : ∀ x y, h (c x y) = c' (g x) (h y)) (x l) : h (f c x l) = f c' (h x) (l.map g) :=
   f.2 (λ x y => g x = y) (λ x y => h x = y) c _ (λ x _ hx y _ hy => hx ▸ hy ▸ hc x y) x _ rfl l _ (lift_map g l)
+
+example : ParaT.prop λ {α β : Type _} x => List.map (λ f : α → β => f x) := by
+  dsimp
+  intro α α' r β β' s x x' hx
+  let rec h : ∀ l l', lift (λ (f : α → β) (g : α' → β') => ∀ x y, r x y → s (f x) (g y)) l l' → lift s (l.map λ f => f x) (l'.map λ g => g x')
+  | [], [], _ => by parametric
+  | _::_, _::_, ⟨_, _⟩ => by parametric h
+  exact h
 
 end List
